using general Map.v from Software Foundations book, implemented Dijkstra

NodeMaps.c
@@ -1,0 +1,104 @@
+(** Total  Map *)
+
+Require Import Arith Bool Graph List FunctionalExtensionality.
+
+Definition adj_map := Node -> nodeList.
+
+Definition adj_empty : Node -> nodeList :=
+  (fun _ => nil).
+
+Definition adj_update (m : adj_map)
+                    (v : Node) (nl : nodeList) :=
+  fun v' => if beq_node v v' then nl else m v'.
+
+(** empty map returns default value*)
+Lemma adj_apply_empty: forall v, adj_empty v = nil.
+Proof.
+  intros.
+  trivial.
+Qed.
+
+(** set and get the same value for same keys*)
+Lemma adj_update_eq : forall (m: adj_map) n nl,
+  (adj_update m n nl) n = nl.
+Proof.
+  intros.
+  unfold adj_update.
+  destruct n.
+  rewrite beq_node_refl.
+  reflexivity.
+Qed.
+
+Theorem adj_update_neq : forall  nl n1 n2
+                         (m : adj_map),
+  n1 <> n2 ->
+  (adj_update m n1 nl) n2 = m n2.
+Proof.
+  intros nl [n1] [n2] m H.
+  unfold adj_update.
+  rewrite -> false_beq_node.
+  trivial.
+  apply H.
+Qed.
+
+(** latest update stays *)
+Lemma adj_update_shadow : forall (m: adj_map) nl1 nl2 n,
+    adj_update (adj_update m n nl1) n nl2
+  = adj_update m n nl2.
+Proof.
+  intros m nl1 nl2 n.
+  unfold adj_update.
+  extensionality x.
+  remember (beq_node n x) as e; induction e.
+  trivial.
+  trivial.
+Qed.
+
+Print reflect.
+Lemma beq_nodeP : forall x y, reflect (x = y) (beq_node x y).
+Proof.
+  intros.
+  apply iff_reflect.
+  rewrite beq_node_true_iff.
+  reflexivity.
+Qed.
+
+(** if we update a map to assign key [x] the same value as it already has in
+    [m], then the result is equal to [m]: *)
+
+Theorem t_update_same : forall n (m : adj_map),
+  adj_update m n (m n) = m.
+Proof.
+  intros.
+  unfold adj_update.
+  extensionality x.
+  remember (beq_node n x) as e; induction e.
+  symmetry in Heqe.
+  apply beq_node_true_iff in Heqe.
+  rewrite Heqe.
+  reflexivity.
+  reflexivity.
+Qed.
+
+(** [] *)
+
+(** If we update a map [m] at two distinct keys, it doesn't
+    matter in which order we do the updates. *)
+Theorem t_update_permute : forall nl1 nl2 n1 n2
+                             (m : adj_map),
+  n2 <> n1 ->
+    (adj_update (adj_update m n2 nl2) n1 nl1)
+  = (adj_update (adj_update m n1 nl1) n2 nl2).
+Proof.
+  intros.
+  unfold adj_update.
+  extensionality x.
+  remember (beq_node n1 x) as e; induction e.
+  symmetry in Heqe.
+  apply beq_node_true_iff in Heqe.
+  rewrite <- Heqe.
+  rewrite -> false_beq_node.
+  reflexivity.
+  exact H.
+  reflexivity.
+Qed.
