Graph.v
@@ -1,12 +1,9 @@
-Require Import List Arith Bool.
+Require Import List Arith Bool Maps FinFun.
 
-Inductive Node : Set :=
-| node : nat ->  Node.
+Module Graph.
 
-Definition beq_node (a : Node) (b : Node) : bool :=
-  match a,b with
-  | node x, node y => beq_nat x y
-  end.
+Inductive node : Set :=
+| Node : nat ->  node.
 
 (*
 Theorem beq_nat_refl : forall n : nat, 
@@ -18,33 +15,51 @@ Proof.
   simpl in |- *; auto.
 Qed. *given in the library*)
 
-Lemma beq_node_refl : forall (n : nat), beq_node (node n) (node n) = true.
+Definition nodeToKeyConverter (n : node) : id :=
+  match n with
+  | Node n => Id n
+  end.
+
+Lemma injectivityOfNodeToKeyConverter : Injective nodeToKeyConverter.
+Proof.
+  unfold Injective.
+  intros.
+  destruct x.
+  destruct y.
+  inversion H.
+  reflexivity.
+Qed.
+
+Definition beq_node (a : node) (b : node) : bool := beq_id (nodeToKeyConverter a) (nodeToKeyConverter b).
+
+Lemma beq_node_refl : forall (a : node), beq_node a a = true.
 Proof.
   intros.
   unfold beq_node.
-  symmetry.
-  apply beq_nat_refl.
+  rewrite beq_id_refl.
+  reflexivity.
 Qed.
 
-Theorem beq_node_true_iff : forall n1 n2 : Node,
+Theorem beq_node_true_iff : forall n1 n2 : node,
   beq_node n1 n2 = true <-> n1 = n2.
 Proof.
    intros [n1] [n2].
    unfold beq_node.
-   rewrite beq_nat_true_iff.
+   rewrite beq_id_true_iff.
+   simpl.
    split.
-   - (* -> *) intros H. rewrite H. reflexivity.
+   - (* -> *) intros H. rewrite injectivityOfNodeToKeyConverter. reflexivity. simpl. exact H.
    - (* <- *) intros H. inversion H. reflexivity.
 Qed.
 
-Theorem beq_node_false_iff : forall x y : Node,
+Theorem beq_node_false_iff : forall x y : node,
   beq_node x y = false
   <-> x <> y.
 Proof.
   intros x y. rewrite <- beq_node_true_iff.
   rewrite not_true_iff_false. reflexivity. Qed.
 
-Theorem false_beq_node : forall x y : Node,
+Theorem false_beq_node : forall x y : node,
    x <> y
    -> beq_node x y = false.
 Proof.
@@ -54,22 +69,70 @@ Proof.
   
 Definition wt := nat.
 
-Inductive Edge : Set :=
-| edge : Node -> Node -> wt -> Edge.
+Inductive edge : Set :=
+| Edge : node -> node -> wt -> edge.
 
-Definition eq_edge (a : Edge) (b : Edge) : bool :=
+Definition eq_edge (a : edge) (b : edge) : bool :=
   match a, b with
-  | edge p q w1, edge r s w2 => andb (beq_nat w1 w2) (andb (beq_node p r) (beq_node q s))                                     
+  | Edge p q w1, Edge r s w2 => andb (beq_node p r) (beq_node q s)                
   end.
 
 
-Definition edgeList := list Edge.
-Definition nodeList := list Node.
+Definition edgeList := list edge.
+Definition nodeList := list node.
 
 
 
-Definition exGraph :=  (edge (node 1) (node 2) 2) ::  (edge (node 2) (node 3) 3) :: nil.
+Definition exGraph := (Edge (Node 1) (Node 2) 2) ::  (Edge (Node 2) (Node 3) 3) :: nil.
 Check exGraph.
+
+(* Define adjacency map, we go for total map as nil is the preferred choice for default rather than None in case of Partial Map*)
+Definition adj_map_empty : total_map nodeList := t_empty nil.
+
+Fixpoint edgeListToAdjMap (el : edgeList) (m : total_map nodeList) : total_map nodeList :=
+  match el with
+  | nil => m
+  | (Edge p q w) :: tl => let pid := (nodeToKeyConverter p) in
+                           edgeListToAdjMap tl (t_update m pid (q::(m pid)))
+end.
+
+Eval compute in (edgeListToAdjMap exGraph adj_map_empty).
+
+(* let's assume 1000 to be the largest weight in any graph *)
+Fixpoint getEdgeWeight (el : edgeList) (e : edge) : wt :=
+  match el with
+  | nil => 1000
+  |  hd :: tl => if eq_edge hd e then
+                  match hd with
+                  | Edge p q w => w
+                  end
+                else getEdgeWeight tl e
+  end.
+
+Definition dist_map : total_map wt := t_empty 1000.
+
+Fixpoint min_dist (dist_map : total_map wt) (minode : node) (q : nodeList) : node :=
+  match q with
+  | nil => minode
+  | hd :: tl => min_dist dist_map (if (dist_map (nodeToKeyConverter hd)) <? (dist_map (nodeToKeyConverter minode)) then hd else minode) tl
+  end.  
+
+Check fold_left.
+
+Fixpoint dijkstra (start_node end_node : node) (adj : total_map nodeList) (q : nodeList) (dist_map : total_map wt) (el : edgeList) (path : nodeList) : prod nodeList wt :=
+  match q with
+  | nil => pair path (dist_map (nodeToKeyConverter end_node))
+  | hd :: tl => let u := min_dist dist_map hd q in
+                let u_neighbours := adj (nodeToKeyConverter u) in
+                 let alt := fun (i : node) => (dist_map (nodeToKeyConverter u)) + getEdgeWeight el (Edge u i 0) in
+                 let updated_dist_map := fold_left (fun (dm : total_map wt) (n : node) => if alt n <? dm (nodeToKeyConverter n) then t_update dm (nodeToKeyConverter n) (alt n) else dm) u_neighbours dist_map in
+                  dijkstra start_node end_node adj tl updated_dist_map el (u::path)
+  end.
+
+Eval compute in dijkstra (Node 1) (Node 3) (edgeListToAdjMap exGraph adj_map_empty) (Node 1 :: Node 2 :: Node 3 :: nil) (t_update dist_map (nodeToKeyConverter (Node 1)) 0) exGraph nil.
+               
+  
+         
 
 
 
